code/nist-pcurves/Hacl.Impl.PCurves.PointMul.fst
@@ -30,7 +30,7 @@ let point_mul_gen {| cp:S.curve_params |} {| bn_ops |} {| curve_constants |} {| 
   let h0 = ST.get () in
   SE.exp_fw_lemma S.mk_pcurve_concrete_ops
     (from_mont_point (as_point_nat h0 p)) cp.bits (as_nat h0 scalar) 4;
-  assert (v (3ul *. cp.bn_limbs) == 3 * v cp.bn_limbs);
-  BE.lexp_fw_consttime (3ul *. cp.bn_limbs) 0ul mk_pcurve_concrete_ops 4ul (null uint64) p cp.bn_limbs (size cp.bits) scalar res
+  assert (v (3ul *! cp.bn_limbs) == 3 * v cp.bn_limbs);
+  BE.lexp_fw_consttime (3ul *! cp.bn_limbs) 0ul mk_pcurve_concrete_ops 4ul (null uint64) p cp.bn_limbs (size cp.bits) scalar res
 
 
