code/nist-pcurves/Hacl.Impl.PCurves.PrecompTable.fst
@@ -45,7 +45,7 @@ let lemma_refl {| cp:S.curve_params |} x =
 
 
 inline_for_extraction noextract
-let mk_pcurve_precomp_base_table {| cp:S.curve_params |} : SPT.mk_precomp_base_table S.proj_point U64 (3ul *. cp.bn_limbs) 0ul = {
+let mk_pcurve_precomp_base_table {| cp:S.curve_params |} : SPT.mk_precomp_base_table S.proj_point U64 (3ul *! cp.bn_limbs) 0ul = {
   SPT.concr_ops = S.mk_pcurve_concrete_ops;
   SPT.to_cm = mk_to_pcurve_comm_monoid;
     SPT.to_list = proj_point_to_list;
@@ -80,7 +80,7 @@ noeq type proj_g_pow2 {| cp:S.curve_params |} (p:S.aff_point #cp) = {
   Lemma (point_inv_seq proj_g_pow2_lseq /\
          S.to_aff_point (from_mont_point
            (as_point_nat_seq proj_g_pow2_lseq)) == p);
-  mk_proj_g_pow2: unit -> StackInline (lbuffer uint64 (3ul *. cp.bn_limbs))
+  mk_proj_g_pow2: unit -> StackInline (lbuffer uint64 (3ul *! cp.bn_limbs))
     (requires fun _ -> True)
     (ensures  fun h0 b h1 -> live h1 b /\ 
               stack_allocated b h0 h1 proj_g_pow2_lseq)
@@ -106,7 +106,7 @@ noeq type precomp_table_w4 {| cp:S.curve_params |} (p:S.aff_point #cp) = {
   table_lseq_w4: (LSeq.lseq uint64 (48 * v cp.bn_limbs));
   table_lemma_w4: unit ->
   Lemma ((forall (i:nat{i < 16}). precomp_table_acc_inv p 16 table_lseq_w4 i));
-  table_w4: x:glbuffer uint64 (48ul *. cp.bn_limbs){witnessed x table_lseq_w4 /\ recallable x}
+  table_w4: x:glbuffer uint64 (48ul *! cp.bn_limbs){witnessed x table_lseq_w4 /\ recallable x}
 }
 
 noextract inline_for_extraction
@@ -114,7 +114,7 @@ noeq type precomp_table_w5 {| cp:S.curve_params |} (p:S.aff_point #cp) = {
   table_lseq_w5: (LSeq.lseq uint64 (96 * v cp.bn_limbs));
   table_lemma_w5: unit ->
   Lemma ((forall (i:nat{i < 32}). precomp_table_acc_inv p 32 table_lseq_w5 i));
-  table_w5: x:glbuffer uint64 (96ul *. cp.bn_limbs){witnessed x table_lseq_w5 /\ recallable x}
+  table_w5: x:glbuffer uint64 (96ul *! cp.bn_limbs){witnessed x table_lseq_w5 /\ recallable x}
 }
 
 open Hacl.Impl.PCurves.Field
@@ -122,14 +122,14 @@ open Hacl.Impl.PCurves.InvSqrt
 open Hacl.Impl.PCurves.Group
 
 inline_for_extraction noextract
-let precomp_get_consttime_t {| cp:S.curve_params |} {| bn_ops |} {| curve_constants |} {| f:field_ops |} {| curve_inv_sqrt|} {| p:point_ops |} = BE.pow_a_to_small_b_st U64 (3ul *. cp.bn_limbs) 0ul mk_pcurve_concrete_ops 4ul 16ul
-    (BE.table_inv_precomp (3ul *. cp.bn_limbs) 0ul mk_pcurve_concrete_ops 4ul 16ul)
+let precomp_get_consttime_t {| cp:S.curve_params |} {| bn_ops |} {| curve_constants |} {| f:field_ops |} {| curve_inv_sqrt|} {| p:point_ops |} = BE.pow_a_to_small_b_st U64 (3ul *! cp.bn_limbs) 0ul mk_pcurve_concrete_ops 4ul 16ul
+    (BE.table_inv_precomp (3ul *! cp.bn_limbs) 0ul mk_pcurve_concrete_ops 4ul 16ul)
 
 inline_for_extraction noextract
 val precomp_get_consttime_gen {| cp:S.curve_params |} {| bn_ops |} {| curve_constants |} {| f:field_ops |} {| curve_inv_sqrt |} {| point_ops |}: precomp_get_consttime_t
 
 let precomp_get_consttime_gen {| cp:S.curve_params |} {| bn_ops |} {| curve_constants |} {| f:field_ops |} {| curve_inv_sqrt |} ctx a table bits_l tmp =
-  [@inline_let] let len = 3ul *. cp.bn_limbs in
+  [@inline_let] let len = 3ul *! cp.bn_limbs in
   [@inline_let] let ctx_len = 0ul in
   [@inline_let] let k = mk_pcurve_concrete_ops in
   [@inline_let] let l = 4ul in
