code/nist-pcurves/Hacl.Impl.PCurves.Group.fsti
@@ -33,7 +33,7 @@ let refl {| cp:S.curve_params |} (p:LSeq.lseq uint64 (3*v cp.bn_limbs){point_inv
 #push-options "--z3rlimit 50"
 [@(strict_on_arguments [0])]
 inline_for_extraction noextract
-let mk_to_pcurve_comm_monoid {| cp:S.curve_params |} : BE.to_comm_monoid U64 (3ul *. cp.bn_limbs) 0ul = {
+let mk_to_pcurve_comm_monoid {| cp:S.curve_params |} : BE.to_comm_monoid U64 (3ul *! cp.bn_limbs) 0ul = {
   BE.a_spec = S.aff_point;
   BE.comm_monoid = S.mk_pcurve_comm_monoid;
   BE.linv_ctx = linv_ctx;
@@ -43,21 +43,21 @@ let mk_to_pcurve_comm_monoid {| cp:S.curve_params |} : BE.to_comm_monoid U64 (3u
 #pop-options
 
 inline_for_extraction noextract
-let point_add_t {| cp:S.curve_params |} {| bn_ops |} {| curve_constants |} {| f:field_ops |} {| curve_inv_sqrt|} = BE.lmul_st U64 (3ul *. cp.bn_limbs) 0ul mk_to_pcurve_comm_monoid
+let point_add_t {| cp:S.curve_params |} {| bn_ops |} {| curve_constants |} {| f:field_ops |} {| curve_inv_sqrt|} = BE.lmul_st U64 (3ul *! cp.bn_limbs) 0ul mk_to_pcurve_comm_monoid
 
 [@(strict_on_arguments [0;1;2;3;4])]
 inline_for_extraction noextract
 val point_add_g {| cp:S.curve_params |} {| bn_ops |} {| curve_constants |} {| f:field_ops |} {| curve_inv_sqrt|} : point_add_t
 
 inline_for_extraction noextract
-let point_double_t {| cp:S.curve_params |} {| bn_ops |} {| curve_constants |} {| f:field_ops |} {| curve_inv_sqrt|} = BE.lsqr_st U64 (3ul *. cp.bn_limbs) 0ul mk_to_pcurve_comm_monoid
+let point_double_t {| cp:S.curve_params |} {| bn_ops |} {| curve_constants |} {| f:field_ops |} {| curve_inv_sqrt|} = BE.lsqr_st U64 (3ul *! cp.bn_limbs) 0ul mk_to_pcurve_comm_monoid
 
 [@(strict_on_arguments [0;1;2;3;4])]
 inline_for_extraction noextract
 val point_double_g {| cp:S.curve_params |} {| bn_ops |} {| curve_constants |} {| f:field_ops |} {| curve_inv_sqrt|}: point_double_t
 
 inline_for_extraction noextract
-let point_zero_t {| cp:S.curve_params |} {| bn_ops |} {| curve_constants |} {| f:field_ops |} {| curve_inv_sqrt|} = BE.lone_st U64 (3ul *. cp.bn_limbs) 0ul mk_to_pcurve_comm_monoid
+let point_zero_t {| cp:S.curve_params |} {| bn_ops |} {| curve_constants |} {| f:field_ops |} {| curve_inv_sqrt|} = BE.lone_st U64 (3ul *! cp.bn_limbs) 0ul mk_to_pcurve_comm_monoid
 
 [@(strict_on_arguments [0;1;2;3;4])]
 inline_for_extraction noextract
@@ -73,7 +73,7 @@ class point_ops {| cp:S.curve_params |} {| bn_ops |} {| curve_constants |} {| fi
 
 [@(strict_on_arguments [0;1;2;3;4;5])]
 inline_for_extraction noextract
-let mk_pcurve_concrete_ops {| S.curve_params |} {| bn_ops |} {| curve_constants |} {| f:field_ops |} {| curve_inv_sqrt|} {| p:point_ops |} : BE.concrete_ops U64 (3ul *. S.bn_limbs) 0ul = {
+let mk_pcurve_concrete_ops {| S.curve_params |} {| bn_ops |} {| curve_constants |} {| f:field_ops |} {| curve_inv_sqrt|} {| p:point_ops |} : BE.concrete_ops U64 (3ul *! S.bn_limbs) 0ul = {
   BE.to = mk_to_pcurve_comm_monoid;
   BE.lone = p.point_zero;
   BE.lmul = p.point_add;
